special case for assume extraction

Loom/MonadAlgebras/NonDetT'/Extract.lean
@@ -130,8 +130,8 @@ inductive ExtractNonDet (findable : {τ : Type u} -> (τ -> Prop) -> Type u) {m}
   | pickSuchThat {α} (τ : Type u) (p : τ -> Prop) (f : τ → NonDetT m α)
     {_ : findable p}
      : (∀ x, ExtractNonDet findable (f x)) → ExtractNonDet findable (.pickCont τ p f)
-  -- | assume {α} (p : PUnit -> Prop) (f : PUnit → NonDetT m α) :
-  --   (∀ x, ExtractNonDet findable (f x)) → ExtractNonDet findable (.pickCont PUnit p f)
+  | assume {α} (p : PUnit -> Prop) (f : PUnit → NonDetT m α) {_ : Decidable (p .unit)} :
+    (∀ x, ExtractNonDet findable (f x)) → ExtractNonDet findable (.pickCont PUnit p f)
 
 set_option linter.unusedVariables false in
 def ExtractNonDet.bind {findable : {τ : Type u} -> (τ -> Prop) -> Type u} :
@@ -144,9 +144,10 @@ def ExtractNonDet.bind {findable : {τ : Type u} -> (τ -> Prop) -> Type u} :
   | .pickSuchThat _ p f inst, inst' => by
     dsimp [Bind.bind, NonDetT.bind]; constructor
     assumption; intro y; apply ExtractNonDet.bind <;> solve_by_elim
-  -- | .assume _ f inst, inst' => by
-  --   dsimp [Bind.bind, NonDetT.bind]; apply ExtractNonDet.assume
-  --   intro y; apply ExtractNonDet.bind <;> solve_by_elim
+  | .assume _ f inst, inst' => by
+    dsimp [Bind.bind, NonDetT.bind];
+    apply ExtractNonDet.assume
+    assumption; intro y; apply ExtractNonDet.bind <;> solve_by_elim
 
 instance ExtractNonDet.pure' : ExtractNonDet findable (Pure.pure (f := NonDetT m) x) := by
   dsimp [Pure.pure, NonDetT.pure]; constructor
@@ -156,9 +157,9 @@ instance ExtractNonDet.liftM (x : m α) :
     dsimp [_root_.liftM, monadLift, MonadLift.monadLift]; constructor
     intro y; apply ExtractNonDet.pure'
 
--- instance ExtractNonDet.assume' {p : Prop} : ExtractNonDet findable (MonadNonDet.assume (m :=  NonDetT m) p) := by
---   dsimp [MonadNonDet.assume, NonDetT.assume]; apply ExtractNonDet.assume
---   intro y; apply ExtractNonDet.pure
+instance ExtractNonDet.assume' {p : Prop} [Decidable p] : ExtractNonDet findable (MonadNonDet.assume (m :=  NonDetT m) p) := by
+  dsimp [MonadNonDet.assume, NonDetT.assume]; apply ExtractNonDet.assume; assumption
+  intro y; apply ExtractNonDet.pure
 
 instance ExtractNonDet.pickSuchThat' {τ : Type u} (p : τ -> Prop) [Findable p] :
   ExtractNonDet Findable (MonadNonDet.pickSuchThat (m := NonDetT m) τ p) := by
@@ -201,7 +202,10 @@ def NonDetT.extractGen {findable : {τ : Type u} -> (τ -> Prop) -> Type u} {α 
     match findOf p ‹_› with
     | none => CCPOBot.compBot
     | some x =>  extractGen findOf (f x)
-  -- | .pickCont _ _ f, .assume _ _ _ => extractGen findOf (f .unit)
+  | .pickCont _ p f, .assume _ _ _ =>
+    if p .unit then
+      extractGen findOf (f .unit)
+    else CCPOBot.compBot
 
 @[inline]
 def NonDetT.extract {α : Type u} (s : NonDetT m α) (ex : ExtractNonDet Findable s := by solve_by_elim) : m α :=
@@ -218,7 +222,7 @@ macro "extract_step" : tactic =>
       | eapply ExtractNonDet.bind
       | eapply ExtractNonDet.pure'
       | eapply ExtractNonDet.liftM
-      -- | eapply ExtractNonDet.assume'
+      | eapply ExtractNonDet.assume'
       | eapply ExtractNonDet.pickSuchThat'
       | eapply ExtractNonDet.pickSuchThat_weak
       | split)
@@ -363,6 +367,10 @@ def ExtractNonDet.prop {α : Type u} (s : NonDetT m α) :  ExtractNonDet WeakFin
   | .pure x => ⊤
   | .vis x f ex => wlp x fun y => (ex y).prop
   | .pickSuchThat _ p f ex => ⨅ t ∈ WeakFindable.find p, (ex t).prop
+  | .assume p f ex =>
+      if p .unit then
+        (ex .unit).prop
+      else ⊤
 
 namespace DemonicChoice
 
@@ -373,16 +381,20 @@ lemma ExtractNonDet.extract_refines_wp (s : NonDetT m α) (inst : ExtractNonDet 
   { simp [NonDetT.wp_vis, NonDetT.prop]; rw [inf_comm, wlp_join_wp]
     simp [NonDetT.extract, wp_bind]
     apply wp_cons; aesop (add norm inf_comm) }
-  simp [NonDetT.wp_pickCont, NonDetT.prop, NonDetT.extract]; split
-  { have := Findable.find_none (p := p) (by simpa);
-    have : (∀ x, p x = False) := by simpa
-    simp [this] }
-  rw [<-inf_assoc]; refine inf_le_of_left_le ?_
-  rw [← @iInf_inf_eq]; simp [meet_himp _ _ _ _ rfl]
-  rename_i y _
-  refine iInf_le_of_le y ?_
-  have := Findable.find_some_p (p := p) (by assumption)
-  simp [this]; apply a_ih
+  { simp [NonDetT.wp_pickCont, NonDetT.prop, NonDetT.extract]; split
+    { have := Findable.find_none (p := p) (by simpa);
+      have : (∀ x, p x = False) := by simpa
+      simp [this] }
+    rw [<-inf_assoc]; refine inf_le_of_left_le ?_
+    rw [← @iInf_inf_eq]; simp [meet_himp _ _ _ _ rfl]
+    rename_i y _
+    refine iInf_le_of_le y ?_
+    have := Findable.find_some_p (p := p) (by assumption)
+    simp [this]; apply a_ih }
+  simp [NonDetT.wp_pickCont, NonDetT.prop, NonDetT.extract]
+  have : ∀ a : PUnit.{u_1 + 1}, a = .unit := by simp
+  simp [this, iInf_const]; split_ifs <;> simp [*, iSup_const]
+  apply a_ih
 
 lemma ExtractNonDet.extract_refines (pre : l) (s : NonDetT m α) (inst : ExtractNonDet Findable s) :
   triple pre s post ->
@@ -415,12 +427,17 @@ lemma ExtractNonDet.extract_refines_wp_weak [CCPOBotLawful m] (s : NonDetT m α)
   { simp [NonDetT.wp_vis, ExtractNonDet.prop];
     simp [NonDetT.extractWeak, wp_bind]
     apply wp_cons; aesop (add norm inf_comm) }
-  simp [NonDetT.wp_pickCont, ExtractNonDet.prop, NonDetT.extractWeak]; split
-  simp [CCPOBotLawful.prop, wp_bot]
-  rename_i y h
-  refine iInf_le_of_le y ?_
-  have := WeakFindable.find_some_p (p := p) (by assumption)
-  simp [this, h]; apply a_ih
+  { simp [NonDetT.wp_pickCont, ExtractNonDet.prop, NonDetT.extractWeak]; split
+    simp [CCPOBotLawful.prop, wp_bot]
+    rename_i y h
+    refine iInf_le_of_le y ?_
+    have := WeakFindable.find_some_p (p := p) (by assumption)
+    simp [this, h]; apply a_ih }
+  simp [NonDetT.wp_pickCont, ExtractNonDet.prop, NonDetT.extractWeak]
+  have : ∀ a : PUnit.{u_1 + 1}, a = .unit := by simp
+  simp [this, iInf_const]; split_ifs <;> simp [*, iSup_const, CCPOBotLawful.prop, wp_bot]
+  apply a_ih
+
 
 omit [MPropDet m l] in
 lemma ExtractNonDet.extract_refines_triple_weak [CCPOBotLawful m] (pre : l) (s : NonDetT m α) (inst : ExtractNonDet WeakFindable s) :
@@ -441,10 +458,14 @@ lemma ExtractNonDet.extract_refines_wp_weak (s : NonDetT m α) (inst : ExtractNo
   { simp [wp_pure, NonDetT.extractWeak] }
   { simp [NonDetT.wp_vis, ExtractNonDet.prop, NonDetT.extractWeak, wp_bind];
     apply wp_cons; aesop (add norm inf_comm) }
-  simp [NonDetT.wp_pickCont, ExtractNonDet.prop, NonDetT.extractWeak]; split
-  { simp [*, CCPOBotLawful.prop, TotalCorrectness.wp_bot] }
-  apply le_iSup_of_le; simp; constructor; rotate_left
-  apply a_ih; rename_i h; simp [x.find_some_p h]
+  { simp [NonDetT.wp_pickCont, ExtractNonDet.prop, NonDetT.extractWeak]; split
+    { simp [*, CCPOBotLawful.prop, TotalCorrectness.wp_bot] }
+    apply le_iSup_of_le; simp; constructor; rotate_left
+    apply a_ih; rename_i h; simp [x.find_some_p h] }
+  simp [NonDetT.wp_pickCont, ExtractNonDet.prop, NonDetT.extractWeak]
+  have : ∀ a : PUnit.{u_1 + 1}, a = .unit := by simp
+  simp [this, iInf_const]; split_ifs <;> simp [*, iSup_const, CCPOBotLawful.prop, TotalCorrectness.wp_bot]
+  apply a_ih
 
 omit [MPropDet m l] in
 lemma ExtractNonDet.extract_refines_triple (pre : l) (s : NonDetT m α) (inst : ExtractNonDet WeakFindable s) :
