Loom/MonadAlgebras/WP/Tactic.lean
@@ -64,7 +64,8 @@ def generateWPStep : TacticM Unit := withMainContext do
 elab "wpgen_app" : tactic => generateWPStep
 macro "wpgen_step" : tactic => `(tactic| first
   | (wpgen_app <;> intros <;> try_resolve_spec_goals)
-  | (intros; split <;> intros))
+  | (intros; split <;> intros)
+  )
 macro "wpgen_intro" : tactic => `(tactic| (apply WPGen.intro; rotate_right))
 macro "wpgen" : tactic => `(tactic| (
   wpgen_intro
